wip

src/Init/Data/Range/Polymorphic/RangeIterator.lean
@@ -27,15 +27,18 @@ This iterator is publicly available via `PRange.iter` after importing
 
 open Std.Iterators
 
-namespace Std.PRange
+namespace Std
+open PRange
+
+namespace Rxc
+
+variable {α : Type u} {lo hi a : α}
 
 /-- Internal state of the range iterators. Do not depend on its internals. -/
 @[unbox]
-structure RangeIterator (shape : BoundShape) (α : Type u) where
+protected structure Iterator (α : Type u) where
   next : Option α
-  upperBound : Bound shape α
-
-variable {α : Type u}
+  upperBound : α
 
 /--
 The pure function mapping a range iterator of type `IterM` to the next step of the iterator.
@@ -43,14 +46,15 @@ The pure function mapping a range iterator of type `IterM` to the next step of t
 This function is prefixed with `Monadic` in order to disambiguate it from the version for iterators
 of type `Iter`.
 -/
-@[always_inline, inline]
-def RangeIterator.Monadic.step {su} [UpwardEnumerable α] [SupportsUpperBound su α]
-    (it : IterM (α := RangeIterator su α) Id α) :
-    IterStep (IterM (α := RangeIterator su α) Id α) α :=
+@[inline]
+def Iterator.Monadic.step [UpwardEnumerable α] [LE α] [DecidableLE α]
+    (it : IterM (α := Rxc.Iterator α) Id α) :
+    IterStep (IterM (α := Rxc.Iterator α) Id α) α :=
   match it.internalState.next with
   | none => .done
-  | some a => if SupportsUpperBound.IsSatisfied it.internalState.upperBound a then
-      .yield ⟨⟨UpwardEnumerable.succ? a, it.internalState.upperBound⟩⟩ a
+  | some next =>
+    if next ≤ it.internalState.upperBound then
+      .yield ⟨⟨UpwardEnumerable.succ? next, it.internalState.upperBound⟩⟩ next
     else
       .done
 
@@ -58,43 +62,43 @@ def RangeIterator.Monadic.step {su} [UpwardEnumerable α] [SupportsUpperBound su
 The pure function mapping a range iterator of type `Iter` to the next step of the iterator.
 -/
 @[always_inline, inline]
-def RangeIterator.step {su} [UpwardEnumerable α] [SupportsUpperBound su α]
-    (it : Iter (α := RangeIterator su α) α) :
-    IterStep (Iter (α := RangeIterator su α) α) α :=
+def Iterator.step [UpwardEnumerable α] [LE α] [DecidableLE α]
+    (it : Iter (α := Rxc.Iterator α) α) :
+    IterStep (Iter (α := Rxc.Iterator α) α) α :=
   match it.internalState.next with
   | none => .done
-  | some a => if SupportsUpperBound.IsSatisfied it.internalState.upperBound a then
-      .yield ⟨⟨UpwardEnumerable.succ? a, it.internalState.upperBound⟩⟩ a
+  | some next => if next ≤ it.internalState.upperBound then
+      .yield ⟨⟨UpwardEnumerable.succ? next, it.internalState.upperBound⟩⟩ next
     else
       .done
 
-theorem RangeIterator.step_eq_monadicStep {su} [UpwardEnumerable α] [SupportsUpperBound su α]
-    {it : Iter (α := RangeIterator su α) α} :
-    RangeIterator.step it = (RangeIterator.Monadic.step it.toIterM).mapIterator IterM.toIter := by
+theorem Iterator.step_eq_monadicStep [UpwardEnumerable α] [LE α] [DecidableLE α]
+    {it : Iter (α := Rxc.Iterator α) α} :
+    Iterator.step it = (Iterator.Monadic.step it.toIterM).mapIterator IterM.toIter := by
   simp only [step, Monadic.step, Iter.toIterM]
   split
   · rfl
   · split <;> rfl
 
 @[always_inline, inline]
-instance {su} [UpwardEnumerable α] [SupportsUpperBound su α] :
-    Iterator (RangeIterator su α) Id α where
-  IsPlausibleStep it step := step = RangeIterator.Monadic.step it
-  step it := pure ⟨RangeIterator.Monadic.step it, rfl⟩
+instance [UpwardEnumerable α] [LE α] [DecidableLE α] :
+    Iterator (Rxc.Iterator α) Id α where
+  IsPlausibleStep it step := step = Iterator.Monadic.step it
+  step it := pure ⟨Iterator.Monadic.step it, rfl⟩
 
-theorem RangeIterator.Monadic.isPlausibleStep_iff {su} [UpwardEnumerable α] [SupportsUpperBound su α]
-    {it : IterM (α := RangeIterator su α) Id α} {step} :
-    it.IsPlausibleStep step ↔ step = RangeIterator.Monadic.step it := by
+theorem Iterator.Monadic.isPlausibleStep_iff [UpwardEnumerable α] [LE α] [DecidableLE α]
+    {it : IterM (α := Rxc.Iterator α) Id α} {step} :
+    it.IsPlausibleStep step ↔ step = Iterator.Monadic.step it := by
   exact Iff.rfl
 
-theorem RangeIterator.Monadic.step_eq_step {su} [UpwardEnumerable α] [SupportsUpperBound su α]
-    {it : IterM (α := RangeIterator su α) Id α} :
-    it.step = pure ⟨RangeIterator.Monadic.step it, isPlausibleStep_iff.mpr rfl⟩ := by
-  simp [IterM.step, Iterator.step]
+theorem Iterator.Monadic.step_eq_step [UpwardEnumerable α] [LE α] [DecidableLE α]
+    {it : IterM (α := Rxc.Iterator α) Id α} :
+    it.step = pure ⟨Iterator.Monadic.step it, isPlausibleStep_iff.mpr rfl⟩ := by
+  simp [IterM.step, Iterators.Iterator.step]
 
-theorem RangeIterator.isPlausibleStep_iff {su} [UpwardEnumerable α] [SupportsUpperBound su α]
-    {it : Iter (α := RangeIterator su α) α} {step} :
-    it.IsPlausibleStep step ↔ step = RangeIterator.step it := by
+theorem Iterator.isPlausibleStep_iff [UpwardEnumerable α] [LE α] [DecidableLE α]
+    {it : Iter (α := Rxc.Iterator α) α} {step} :
+    it.IsPlausibleStep step ↔ step = Iterator.step it := by
   simp only [Iter.IsPlausibleStep, Monadic.isPlausibleStep_iff, step_eq_monadicStep]
   constructor
   · intro h
@@ -105,33 +109,33 @@ theorem RangeIterator.isPlausibleStep_iff {su} [UpwardEnumerable α] [SupportsUp
   · rintro rfl
     simp only [IterStep.mapIterator_mapIterator, Iter.toIterM_comp_toIter, IterStep.mapIterator_id]
 
-theorem RangeIterator.step_eq_step {su} [UpwardEnumerable α] [SupportsUpperBound su α]
-    {it : Iter (α := RangeIterator su α) α} :
-    it.step = ⟨RangeIterator.step it, isPlausibleStep_iff.mpr rfl⟩ := by
+theorem Iterator.step_eq_step [UpwardEnumerable α] [LE α] [DecidableLE α]
+    {it : Iter (α := Rxc.Iterator α) α} :
+    it.step = ⟨Iterator.step it, isPlausibleStep_iff.mpr rfl⟩ := by
   simp [Iter.step, step_eq_monadicStep, Monadic.step_eq_step, IterM.Step.toPure]
 
-instance RangeIterator.instIteratorCollect {su} [UpwardEnumerable α] [SupportsUpperBound su α]
-    {n : Type u → Type w} [Monad n] : IteratorCollect (RangeIterator su α) Id n :=
+instance Iterator.instIteratorCollect [UpwardEnumerable α] [LE α] [DecidableLE α]
+    {n : Type u → Type w} [Monad n] : IteratorCollect (Rxc.Iterator α) Id n :=
   .defaultImplementation
 
-instance RangeIterator.instIteratorCollectPartial {su} [UpwardEnumerable α] [SupportsUpperBound su α]
-    {n : Type u → Type w} [Monad n] : IteratorCollectPartial (RangeIterator su α) Id n :=
+instance Iterator.instIteratorCollectPartial [UpwardEnumerable α] [LE α] [DecidableLE α]
+    {n : Type u → Type w} [Monad n] : IteratorCollectPartial (Rxc.Iterator α) Id n :=
   .defaultImplementation
 
-theorem RangeIterator.Monadic.isPlausibleOutput_next {su a}
-    [UpwardEnumerable α] [SupportsUpperBound su α]
-    {it : IterM (α := RangeIterator su α) Id α} (h : it.internalState.next = some a)
-    (hP : SupportsUpperBound.IsSatisfied it.internalState.upperBound a) :
+theorem Iterator.Monadic.isPlausibleOutput_next {a}
+    [UpwardEnumerable α] [LE α] [DecidableLE α]
+    {it : IterM (α := Rxc.Iterator α) Id α} (h : it.internalState.next = some a)
+    (hP : a ≤ it.internalState.upperBound) :
     it.IsPlausibleOutput a := by
-  simp [IterM.IsPlausibleOutput, Monadic.isPlausibleStep_iff, RangeIterator.Monadic.step, h, hP]
+  simp [IterM.IsPlausibleOutput, Monadic.isPlausibleStep_iff, Monadic.step, h, hP]
 
-theorem RangeIterator.Monadic.isPlausibleOutput_iff {su a}
-    [UpwardEnumerable α] [SupportsUpperBound su α]
-    {it : IterM (α := RangeIterator su α) Id α} :
+theorem Iterator.Monadic.isPlausibleOutput_iff
+    [UpwardEnumerable α] [LE α] [DecidableLE α]
+    {it : IterM (α := Rxc.Iterator α) Id α} :
     it.IsPlausibleOutput a ↔
       it.internalState.next = some a ∧
-        SupportsUpperBound.IsSatisfied it.internalState.upperBound a := by
-  simp [IterM.IsPlausibleOutput, isPlausibleStep_iff, RangeIterator.Monadic.step]
+        a ≤ it.internalState.upperBound := by
+  simp [IterM.IsPlausibleOutput, isPlausibleStep_iff, Monadic.step]
   split
   · simp [*]
   · constructor
@@ -142,34 +146,34 @@ theorem RangeIterator.Monadic.isPlausibleOutput_iff {su a}
       simp only [heq', Option.some.injEq] at heq
       simp_all
 
-theorem RangeIterator.isPlausibleOutput_next {su a}
-    [UpwardEnumerable α] [SupportsUpperBound su α]
-    {it : Iter (α := RangeIterator su α) α} (h : it.internalState.next = some a)
-    (hP : SupportsUpperBound.IsSatisfied it.internalState.upperBound a) :
+theorem Iterator.isPlausibleOutput_next
+    [UpwardEnumerable α] [LE α] [DecidableLE α]
+    {it : Iter (α := Rxc.Iterator α) α} (h : it.internalState.next = some a)
+    (hP : a ≤ it.internalState.upperBound) :
     it.IsPlausibleOutput a := by
   simp [Iter.IsPlausibleOutput, Monadic.isPlausibleOutput_iff, Iter.toIterM, h, hP]
 
-theorem RangeIterator.isPlausibleOutput_iff {su a}
-    [UpwardEnumerable α] [SupportsUpperBound su α]
-    {it : Iter (α := RangeIterator su α) α} :
+theorem Iterator.isPlausibleOutput_iff
+    [UpwardEnumerable α] [LE α] [DecidableLE α]
+    {it : Iter (α := Rxc.Iterator α) α} :
     it.IsPlausibleOutput a ↔
       it.internalState.next = some a ∧
-        SupportsUpperBound.IsSatisfied it.internalState.upperBound a := by
+        a ≤ it.internalState.upperBound := by
   simp [Iter.IsPlausibleOutput, Monadic.isPlausibleOutput_iff, Iter.toIterM]
 
-theorem RangeIterator.Monadic.isPlausibleSuccessorOf_iff {su}
-    [UpwardEnumerable α] [SupportsUpperBound su α]
-    {it' it : IterM (α := RangeIterator su α) Id α} :
+theorem Iterator.Monadic.isPlausibleSuccessorOf_iff
+    [UpwardEnumerable α] [LE α] [DecidableLE α]
+    {it' it : IterM (α := Rxc.Iterator α) Id α} :
     it'.IsPlausibleSuccessorOf it ↔
       ∃ a, it.internalState.next = some a ∧
-        SupportsUpperBound.IsSatisfied it.internalState.upperBound a ∧
+        a ≤ it.internalState.upperBound ∧
         UpwardEnumerable.succ? a = it'.internalState.next ∧
         it'.internalState.upperBound = it.internalState.upperBound := by
   simp only [IterM.IsPlausibleSuccessorOf]
   constructor
   · rintro ⟨step, h, h'⟩
     cases h'
-    simp only [RangeIterator.Monadic.step] at h
+    simp only [Monadic.step] at h
     split at h
     · cases h
     · split at h
@@ -183,20 +187,19 @@ theorem RangeIterator.Monadic.isPlausibleSuccessorOf_iff {su}
       IterStep.yield.injEq, and_true]
     simp [h'.1, ← h'.2]
 
-theorem RangeIterator.isPlausibleSuccessorOf_iff {su}
-    [UpwardEnumerable α] [SupportsUpperBound su α]
-    {it' it : Iter (α := RangeIterator su α) α} :
+theorem Iterator.isPlausibleSuccessorOf_iff
+    [UpwardEnumerable α] [LE α] [DecidableLE α]
+    {it' it : Iter (α := Rxc.Iterator α) α} :
     it'.IsPlausibleSuccessorOf it ↔
       ∃ a, it.internalState.next = some a ∧
-        SupportsUpperBound.IsSatisfied it.internalState.upperBound a ∧
+        a ≤ it.internalState.upperBound ∧
         UpwardEnumerable.succ? a = it'.internalState.next ∧
         it'.internalState.upperBound = it.internalState.upperBound := by
   simp [Iter.IsPlausibleSuccessorOf, Monadic.isPlausibleSuccessorOf_iff, Iter.toIterM]
 
-theorem RangeIterator.isSome_next_of_isPlausibleIndirectOutput {su}
-    [UpwardEnumerable α] [SupportsUpperBound su α]
-    {it : Iter (α := RangeIterator su α) α} {out : α}
-    (h : it.IsPlausibleIndirectOutput out) :
+theorem Iterator.isSome_next_of_isPlausibleIndirectOutput
+    [UpwardEnumerable α] [LE α] [DecidableLE α]
+    {it : Iter (α := Rxc.Iterator α) α} {out : α} (h : it.IsPlausibleIndirectOutput out) :
     it.internalState.next.isSome := by
   cases h
   case direct h =>
@@ -229,14 +232,14 @@ private def List.length_filter_strict_mono {l : List α} {P Q : α → Bool} {a 
     rw [← heq, List.mem_filter] at this
     exact this.2
 
-private def RangeIterator.instFinitenessRelation [UpwardEnumerable α] [SupportsUpperBound su α]
-    [LawfulUpwardEnumerable α] [HasFiniteRanges su α] :
-    FinitenessRelation (RangeIterator su α) Id where
+private def Iterator.instFinitenessRelation [UpwardEnumerable α] [LE α] [DecidableLE α]
+    [LawfulUpwardEnumerable α] [Rxc.IsAlwaysFinite α] :
+    FinitenessRelation (Rxc.Iterator α) Id where
   rel it' it := it'.IsPlausibleSuccessorOf it
   wf := by
     constructor
     intro it
-    have hnone : ∀ bound, Acc (fun it' it : IterM (α := RangeIterator su α) Id α => it'.IsPlausibleSuccessorOf it)
+    have hnone : ∀ bound, Acc (fun it' it : IterM (α := Rxc.Iterator α) Id α => it'.IsPlausibleSuccessorOf it)
         ⟨⟨none, bound⟩⟩ := by
       intro bound
       constructor
@@ -248,7 +251,7 @@ private def RangeIterator.instFinitenessRelation [UpwardEnumerable α] [Supports
     match it with
     | ⟨⟨none, _⟩⟩ => apply hnone
     | ⟨⟨some init, bound⟩⟩ =>
-      obtain ⟨n, hn⟩ := HasFiniteRanges.finite init bound
+      obtain ⟨n, hn⟩ := Rxc.IsAlwaysFinite.finite init bound
       induction n generalizing init with
       | zero =>
         simp only [succMany?_zero, Option.elim_some] at hn
@@ -277,14 +280,14 @@ private def RangeIterator.instFinitenessRelation [UpwardEnumerable α] [Supports
   subrelation := id
 
 @[no_expose]
-instance RangeIterator.instFinite {su} [UpwardEnumerable α] [SupportsUpperBound su α]
-    [LawfulUpwardEnumerable α] [HasFiniteRanges su α] :
-    Finite (RangeIterator su α) Id :=
+instance Iterator.instFinite [UpwardEnumerable α] [LE α] [DecidableLE α]
+    [LawfulUpwardEnumerable α] [Rxc.IsAlwaysFinite α] :
+    Finite (Rxc.Iterator α) Id :=
   .of_finitenessRelation instFinitenessRelation
 
-private def RangeIterator.instProductivenessRelation [UpwardEnumerable α] [SupportsUpperBound su α]
+private def Iterator.instProductivenessRelation [UpwardEnumerable α] [LE α] [DecidableLE α]
     [LawfulUpwardEnumerable α] :
-    ProductivenessRelation (RangeIterator su α) Id where
+    ProductivenessRelation (Rxc.Iterator α) Id where
   rel := emptyWf.rel
   wf := emptyWf.wf
   subrelation {it it'} h := by
@@ -298,17 +301,17 @@ private def RangeIterator.instProductivenessRelation [UpwardEnumerable α] [Supp
       · cases h
 
 @[no_expose]
-instance RangeIterator.instProductive {su} [UpwardEnumerable α] [SupportsUpperBound su α]
+instance Iterator.instProductive [UpwardEnumerable α] [LE α] [DecidableLE α]
     [LawfulUpwardEnumerable α] :
-    Productive (RangeIterator su α) Id :=
+    Productive (Rxc.Iterator α) Id :=
   .of_productivenessRelation instProductivenessRelation
 
-instance RangeIterator.instIteratorAccess {su} [UpwardEnumerable α] [SupportsUpperBound su α]
-    [LawfulUpwardEnumerable α] [LawfulUpwardEnumerableUpperBound su α] :
-    IteratorAccess (RangeIterator su α) Id where
+instance Iterator.instIteratorAccess [UpwardEnumerable α] [LE α] [DecidableLE α]
+    [LawfulUpwardEnumerable α] [LawfulUpwardEnumerableLE α] [Trans (α := α) (· ≤ ·) (· ≤ ·) (· ≤ ·)] :
+    IteratorAccess (Rxc.Iterator α) Id where
   nextAtIdx? it n := ⟨match it.internalState.next.bind (UpwardEnumerable.succMany? n) with
     | none => .done
-    | some next => if SupportsUpperBound.IsSatisfied it.internalState.upperBound next then
+    | some next => if next ≤ it.internalState.upperBound then
         .yield ⟨⟨UpwardEnumerable.succ? next, it.internalState.upperBound⟩⟩ next
       else
         .done, (by
@@ -341,7 +344,7 @@ instance RangeIterator.instIteratorAccess {su} [UpwardEnumerable α] [SupportsUp
             simp only [heq', Option.bind_some, succMany?_succ?_eq_succ?_bind_succMany?] at heq
             specialize ih ⟨⟨UpwardEnumerable.succ? out, it.internalState.upperBound⟩⟩
             simp only [heq] at ih
-            by_cases heq'' : SupportsUpperBound.IsSatisfied it.internalState.upperBound out
+            by_cases heq'' : out ≤ it.internalState.upperBound
             · apply IterM.IsPlausibleNthOutputStep.yield
               · simp only [Monadic.isPlausibleStep_iff, Monadic.step, heq', heq'', ↓reduceIte,
                 IterStep.yield.injEq]
@@ -357,37 +360,40 @@ instance RangeIterator.instIteratorAccess {su} [UpwardEnumerable α] [SupportsUp
           simp only [succMany?_succ?_eq_succ?_bind_succMany?] at heq
           specialize ih ⟨⟨UpwardEnumerable.succ? out, it.internalState.upperBound⟩⟩
           simp only [heq] at ih
-          by_cases hout : SupportsUpperBound.IsSatisfied it.internalState.upperBound out
+          by_cases hout : out ≤ it.internalState.upperBound
           · apply IterM.IsPlausibleNthOutputStep.yield
             · simp only [Monadic.isPlausibleStep_iff, Monadic.step, heq', hout, ↓reduceIte,
               IterStep.yield.injEq]
               exact ⟨rfl, rfl⟩
             · apply ih
-          · have := hout.imp (fun h => LawfulUpwardEnumerableUpperBound.isSatisfied_of_le _ _ _ h hle)
+          · rename_i next
+            have := hout.imp (fun h : next ≤ it.internalState.upperBound => by
+              rw [← UpwardEnumerable.le_iff] at hle
+              exact Trans.trans hle h)
             simp only [this, ↓reduceIte]
             simp only [this, ↓reduceIte] at ih
             apply IterM.IsPlausibleNthOutputStep.done
             simp [Monadic.isPlausibleStep_iff, Monadic.step, heq', hout])⟩
 
-instance RangeIterator.instLawfulDeterministicIterator {su} [UpwardEnumerable α] [SupportsUpperBound su α] :
-    LawfulDeterministicIterator (RangeIterator su α) Id where
+instance Iterator.instLawfulDeterministicIterator [UpwardEnumerable α] [LE α] [DecidableLE α] :
+    LawfulDeterministicIterator (Rxc.Iterator α) Id where
   isPlausibleStep_eq_eq it := ⟨Monadic.step it, rfl⟩
 
-theorem RangeIterator.Monadic.isPlausibleIndirectOutput_iff {su α}
-    [UpwardEnumerable α] [SupportsUpperBound su α]
-    [LawfulUpwardEnumerable α] [LawfulUpwardEnumerableUpperBound su α]
-    {it : IterM (α := RangeIterator su α) Id α} {out : α} :
+theorem Iterator.Monadic.isPlausibleIndirectOutput_iff
+    [UpwardEnumerable α] [LE α] [DecidableLE α] [LawfulUpwardEnumerableLE α]
+    [LawfulUpwardEnumerable α] [Trans (α := α) (· ≤ ·) (· ≤ ·) (· ≤ ·)]
+    {it : IterM (α := Rxc.Iterator α) Id α} {out : α} :
     it.IsPlausibleIndirectOutput out ↔
       ∃ n, it.internalState.next.bind (succMany? n ·) = some out ∧
-        SupportsUpperBound.IsSatisfied it.internalState.upperBound out := by
+        out ≤ it.internalState.upperBound := by
   constructor
   · intro h
     induction h
     case direct h =>
-      rw [RangeIterator.Monadic.isPlausibleOutput_iff] at h
+      rw [Monadic.isPlausibleOutput_iff] at h
       refine ⟨0, by simp [h, LawfulUpwardEnumerable.succMany?_zero]⟩
     case indirect h _ ih =>
-      rw [RangeIterator.Monadic.isPlausibleSuccessorOf_iff] at h
+      rw [Monadic.isPlausibleSuccessorOf_iff] at h
       obtain ⟨n, hn⟩ := ih
       obtain ⟨a, ha, h₁, h₂, h₃⟩ := h
       refine ⟨n + 1, ?_⟩
@@ -396,7 +402,7 @@ theorem RangeIterator.Monadic.isPlausibleIndirectOutput_iff {su α}
     induction n generalizing it
     case zero =>
       apply IterM.IsPlausibleIndirectOutput.direct
-      rw [RangeIterator.Monadic.isPlausibleOutput_iff]
+      rw [Monadic.isPlausibleOutput_iff]
       exact ⟨by simpa [LawfulUpwardEnumerable.succMany?_zero] using hn, hu⟩
     case succ ih =>
       cases hn' : it.internalState.next
@@ -411,19 +417,17 @@ theorem RangeIterator.Monadic.isPlausibleIndirectOutput_iff {su α}
       simp only [hn', Option.bind_some] at hn
       specialize ih (it := ⟨some a', it.internalState.upperBound⟩) hn hu
       refine IterM.IsPlausibleIndirectOutput.indirect ?_ ih
-      rw [RangeIterator.Monadic.isPlausibleSuccessorOf_iff]
+      rw [Monadic.isPlausibleSuccessorOf_iff]
       refine ⟨a, ‹_›, ?_, hn', rfl⟩
-      apply LawfulUpwardEnumerableUpperBound.isSatisfied_of_le _ a out
-      · exact hu
-      · exact hle
+      exact Trans.trans (α := α) (r := (· ≤ ·)) (UpwardEnumerable.le_iff.mpr hle) hu
 
-theorem RangeIterator.isPlausibleIndirectOutput_iff {su α}
-    [UpwardEnumerable α] [SupportsUpperBound su α]
-    [LawfulUpwardEnumerable α] [LawfulUpwardEnumerableUpperBound su α]
-    {it : Iter (α := RangeIterator su α) α} {out : α} :
+theorem Iterator.isPlausibleIndirectOutput_iff
+    [UpwardEnumerable α] [LE α] [DecidableLE α] [Trans (α := α) (· ≤ ·) (· ≤ ·) (· ≤ ·)]
+    [LawfulUpwardEnumerable α] [LawfulUpwardEnumerableLE α]
+    {it : Iter (α := Rxc.Iterator α) α} {out : α} :
     it.IsPlausibleIndirectOutput out ↔
       ∃ n, it.internalState.next.bind (succMany? n ·) = some out ∧
-        SupportsUpperBound.IsSatisfied it.internalState.upperBound out := by
+        out ≤ it.internalState.upperBound := by
   simp only [Iter.isPlausibleIndirectOutput_iff_isPlausibleIndirectOutput_toIterM,
     Monadic.isPlausibleIndirectOutput_iff, Iter.toIterM]
 
@@ -436,28 +440,28 @@ loop implementation.
 -/
 
 @[always_inline, inline]
-instance RangeIterator.instIteratorLoop {su} [UpwardEnumerable α] [SupportsUpperBound su α]
-    [LawfulUpwardEnumerable α] [LawfulUpwardEnumerableUpperBound su α]
+instance Iterator.instIteratorLoop [UpwardEnumerable α] [LE α] [DecidableLE α]
+    [LawfulUpwardEnumerable α] [LawfulUpwardEnumerableLE α] [Trans (α := α) (· ≤ ·) (· ≤ ·) (· ≤ ·)]
     {n : Type u → Type w} [Monad n] :
-    IteratorLoop (RangeIterator su α) Id n where
+    IteratorLoop (Rxc.Iterator α) Id n where
   forIn _ γ Pl wf it init f :=
     match it with
     | ⟨⟨some next, upperBound⟩⟩ =>
-      if hu : SupportsUpperBound.IsSatisfied upperBound next then
+      if hu : next ≤ upperBound then
         loop γ Pl wf upperBound next init (fun a ha₁ ha₂ c => f a ?hf c) next ?hle hu
       else
         return init
     | ⟨⟨none, _⟩⟩ => return init
   where
     @[specialize]
-    loop γ Pl wf (upperBound : Bound su α) least acc
-        (f : (out : α) → UpwardEnumerable.LE least out → SupportsUpperBound.IsSatisfied upperBound out → (c : γ) → n (Subtype (fun s : ForInStep γ => Pl out c s)))
-        (next : α) (hl : UpwardEnumerable.LE least next) (hu : SupportsUpperBound.IsSatisfied upperBound next) : n γ := do
+    loop γ Pl wf (upperBound : α) least acc
+        (f : (out : α) → UpwardEnumerable.LE least out → out ≤ upperBound → (c : γ) → n (Subtype (fun s : ForInStep γ => Pl out c s)))
+        (next : α) (hl : UpwardEnumerable.LE least next) (hu : next ≤ upperBound) : n γ := do
       match ← f next hl hu acc with
       | ⟨.yield acc', _⟩ =>
         match hs : UpwardEnumerable.succ? next with
         | some next' =>
-          if hu : SupportsUpperBound.IsSatisfied upperBound next' then
+          if hu : next' ≤ upperBound then
             loop γ Pl wf upperBound least acc' f next' ?hle' hu
           else
             return acc'
@@ -465,11 +469,11 @@ instance RangeIterator.instIteratorLoop {su} [UpwardEnumerable α] [SupportsUppe
       | ⟨.done acc', _⟩ => return acc'
     termination_by IteratorLoop.WithWF.mk ⟨⟨some next, upperBound⟩⟩ acc (hwf := wf)
     decreasing_by
-      simp [IteratorLoop.rel, RangeIterator.Monadic.isPlausibleStep_iff,
-        RangeIterator.Monadic.step, *]
+      simp [IteratorLoop.rel, Monadic.isPlausibleStep_iff,
+        Monadic.step, *]
   finally
     case hf =>
-      rw [RangeIterator.Monadic.isPlausibleIndirectOutput_iff]
+      rw [Monadic.isPlausibleIndirectOutput_iff]
       obtain ⟨n, hn⟩ := ha₁
       exact ⟨n, hn, ha₂⟩
     case hle =>
@@ -478,27 +482,27 @@ instance RangeIterator.instIteratorLoop {su} [UpwardEnumerable α] [SupportsUppe
       refine UpwardEnumerable.le_trans hl ⟨1, ?_⟩
       simp [succMany?_one, hs]
 
-partial instance RepeatIterator.instIteratorLoopPartial {su} [UpwardEnumerable α]
-    [SupportsUpperBound su α] [LawfulUpwardEnumerable α] [LawfulUpwardEnumerableUpperBound su α]
-    {n : Type u → Type w} [Monad n] : IteratorLoopPartial (RangeIterator su α) Id n where
+partial instance Iterator.instIteratorLoopPartial [UpwardEnumerable α] [LE α] [DecidableLE α]
+    [LawfulUpwardEnumerable α] [LawfulUpwardEnumerableLE α] [Trans (α := α) (· ≤ ·) (· ≤ ·) (· ≤ ·)]
+    {n : Type u → Type w} [Monad n] : IteratorLoopPartial (Rxc.Iterator α) Id n where
   forInPartial _ γ it init f :=
     match it with
     | ⟨⟨some next, upperBound⟩⟩ =>
-      if hu : SupportsUpperBound.IsSatisfied upperBound next then
+      if hu : next ≤ upperBound then
         loop γ upperBound next init (fun a ha₁ ha₂ c => f a ?hf c) next ?hle hu
       else
         return init
     | ⟨⟨none, _⟩⟩ => return init
   where
     @[specialize]
-    loop γ (upperBound : Bound su α) least acc
-        (f : (out : α) → UpwardEnumerable.LE least out → SupportsUpperBound.IsSatisfied upperBound out → (c : γ) → n (ForInStep γ))
-        (next : α) (hl : UpwardEnumerable.LE least next) (hu : SupportsUpperBound.IsSatisfied upperBound next) : n γ := do
+    loop γ (upperBound : α) least acc
+        (f : (out : α) → UpwardEnumerable.LE least out → out ≤ upperBound → (c : γ) → n (ForInStep γ))
+        (next : α) (hl : UpwardEnumerable.LE least next) (hu : next ≤ upperBound) : n γ := do
       match ← f next hl hu acc with
       | .yield acc' =>
         match hs : succ? next with
         | some next' =>
-          if hu : SupportsUpperBound.IsSatisfied upperBound next' then
+          if hu : next' ≤ upperBound then
             loop γ upperBound least acc' f next' ?hle' hu
           else
             return acc'
@@ -506,7 +510,7 @@ partial instance RepeatIterator.instIteratorLoopPartial {su} [UpwardEnumerable �
       | .done acc' => return acc'
   finally
     case hf =>
-      rw [RangeIterator.Monadic.isPlausibleIndirectOutput_iff]
+      rw [Monadic.isPlausibleIndirectOutput_iff]
       obtain ⟨n, hn⟩ := ha₁
       exact ⟨n, hn, ha₂⟩
     case hle =>
@@ -515,26 +519,26 @@ partial instance RepeatIterator.instIteratorLoopPartial {su} [UpwardEnumerable �
       refine UpwardEnumerable.le_trans hl ⟨1, ?_⟩
       simp [succMany?_one, hs]
 
-theorem RangeIterator.instIteratorLoop.loop_eq {su} [UpwardEnumerable α]
-    [SupportsUpperBound su α] [LawfulUpwardEnumerable α] [LawfulUpwardEnumerableUpperBound su α]
+theorem Iterator.instIteratorLoop.loop_eq [UpwardEnumerable α] [LE α] [DecidableLE α]
+    [LawfulUpwardEnumerable α] [LawfulUpwardEnumerableLE α] [Trans (α := α) (· ≤ ·) (· ≤ ·) (· ≤ ·)]
     {n : Type u → Type w} [Monad n] [LawfulMonad n] {γ : Type u}
     {lift} [Internal.LawfulMonadLiftBindFunction lift]
     {PlausibleForInStep} {upperBound} {next} {hl} {hu} {f} {acc} {wf} :
-    loop (α := α) (su := su) (n := n) γ PlausibleForInStep wf upperBound least acc f next hl hu =
+    loop (α := α) (n := n) γ PlausibleForInStep wf upperBound least acc f next hl hu =
       (do
         match ← f next hl hu acc with
         | ⟨.yield c, _⟩ =>
-          letI it' : IterM (α := RangeIterator su α) Id α := ⟨⟨succ? next, upperBound⟩⟩
+          letI it' : IterM (α := Rxc.Iterator α) Id α := ⟨⟨succ? next, upperBound⟩⟩
           IterM.DefaultConsumers.forIn' (m := Id) lift γ
             PlausibleForInStep wf it' c it'.IsPlausibleIndirectOutput (fun _ => id)
             (fun b h c => f b
                 (by
                   refine UpwardEnumerable.le_trans hl ?_
-                  simp only [RangeIterator.Monadic.isPlausibleIndirectOutput_iff, it',
+                  simp only [Monadic.isPlausibleIndirectOutput_iff, it',
                     ← succMany?_succ?_eq_succ?_bind_succMany?] at h
                   exact ⟨h.choose + 1, h.choose_spec.1⟩)
                 (by
-                  simp only [RangeIterator.Monadic.isPlausibleIndirectOutput_iff, it'] at h
+                  simp only [Monadic.isPlausibleIndirectOutput_iff, it'] at h
                   exact h.choose_spec.2) c)
         | ⟨.done c, _⟩ => return c) := by
   rw [loop]
@@ -564,19 +568,18 @@ theorem RangeIterator.instIteratorLoop.loop_eq {su} [UpwardEnumerable α]
   · simp
 termination_by IteratorLoop.WithWF.mk ⟨⟨some next, upperBound⟩⟩ acc (hwf := wf)
 decreasing_by
-      simp [IteratorLoop.rel, RangeIterator.Monadic.isPlausibleStep_iff,
-        RangeIterator.Monadic.step, *]
+      simp [IteratorLoop.rel, Monadic.isPlausibleStep_iff, Monadic.step, *]
 
-instance RangeIterator.instLawfulIteratorLoop {su} [UpwardEnumerable α] [SupportsUpperBound su α]
-    [LawfulUpwardEnumerable α] [LawfulUpwardEnumerableUpperBound su α]
+instance Iterator.instLawfulIteratorLoop [UpwardEnumerable α] [LE α] [DecidableLE α]
+    [LawfulUpwardEnumerable α] [LawfulUpwardEnumerableLE α] [Trans (α := α) (· ≤ ·) (· ≤ ·) (· ≤ ·)]
     {n : Type u → Type w} [Monad n] [LawfulMonad n] :
-    LawfulIteratorLoop (RangeIterator su α) Id n where
+    LawfulIteratorLoop (Rxc.Iterator α) Id n where
   lawful := by
     intro lift instLawfulMonadLiftFunction
     ext γ PlausibleForInStep hwf it init f
     simp only [IteratorLoop.forIn, IteratorLoop.defaultImplementation]
     rw [IterM.DefaultConsumers.forIn']
-    simp only [RangeIterator.Monadic.step_eq_step, RangeIterator.Monadic.step]
+    simp only [Monadic.step_eq_step, Monadic.step]
     simp only [Internal.LawfulMonadLiftBindFunction.liftBind_pure]
     split
     · rename_i it f next upperBound f'
@@ -594,4 +597,1066 @@ instance RangeIterator.instLawfulIteratorLoop {su} [UpwardEnumerable α] [Suppor
       · simp
     · simp
 
-end Std.PRange.IteratorLoop
+end IteratorLoop
+
+end Rxc
+
+namespace Rxo
+
+variable {α : Type u} {lo hi a : α}
+
+/-- Internal state of the range iterators. Do not depend on its internals. -/
+@[unbox]
+protected structure Iterator (α : Type u) where
+  next : Option α
+  upperBound : α
+
+/--
+The pure function mapping a range iterator of type `IterM` to the next step of the iterator.
+
+This function is prefixed with `Monadic` in order to disambiguate it from the version for iterators
+of type `Iter`.
+-/
+@[inline]
+def Iterator.Monadic.step [UpwardEnumerable α] [LT α] [DecidableLT α]
+    (it : IterM (α := Rxo.Iterator α) Id α) :
+    IterStep (IterM (α := Rxo.Iterator α) Id α) α :=
+  match it.internalState.next with
+  | none => .done
+  | some next =>
+    if next < it.internalState.upperBound then
+      .yield ⟨⟨UpwardEnumerable.succ? next, it.internalState.upperBound⟩⟩ next
+    else
+      .done
+
+/--
+The pure function mapping a range iterator of type `Iter` to the next step of the iterator.
+-/
+@[always_inline, inline]
+def Iterator.step [UpwardEnumerable α] [LT α] [DecidableLT α]
+    (it : Iter (α := Rxo.Iterator α) α) :
+    IterStep (Iter (α := Rxo.Iterator α) α) α :=
+  match it.internalState.next with
+  | none => .done
+  | some next => if next < it.internalState.upperBound then
+      .yield ⟨⟨UpwardEnumerable.succ? next, it.internalState.upperBound⟩⟩ next
+    else
+      .done
+
+theorem Iterator.step_eq_monadicStep [UpwardEnumerable α] [LT α] [DecidableLT α]
+    {it : Iter (α := Rxo.Iterator α) α} :
+    Iterator.step it = (Iterator.Monadic.step it.toIterM).mapIterator IterM.toIter := by
+  simp only [step, Monadic.step, Iter.toIterM]
+  split
+  · rfl
+  · split <;> rfl
+
+@[always_inline, inline]
+instance [UpwardEnumerable α] [LT α] [DecidableLT α] :
+    Iterator (Rxo.Iterator α) Id α where
+  IsPlausibleStep it step := step = Iterator.Monadic.step it
+  step it := pure ⟨Iterator.Monadic.step it, rfl⟩
+
+theorem Iterator.Monadic.isPlausibleStep_iff [UpwardEnumerable α] [LT α] [DecidableLT α]
+    {it : IterM (α := Rxo.Iterator α) Id α} {step} :
+    it.IsPlausibleStep step ↔ step = Iterator.Monadic.step it := by
+  exact Iff.rfl
+
+theorem Iterator.Monadic.step_eq_step [UpwardEnumerable α] [LT α] [DecidableLT α]
+    {it : IterM (α := Rxo.Iterator α) Id α} :
+    it.step = pure ⟨Iterator.Monadic.step it, isPlausibleStep_iff.mpr rfl⟩ := by
+  simp [IterM.step, Iterators.Iterator.step]
+
+theorem Iterator.isPlausibleStep_iff [UpwardEnumerable α] [LT α] [DecidableLT α]
+    {it : Iter (α := Rxo.Iterator α) α} {step} :
+    it.IsPlausibleStep step ↔ step = Iterator.step it := by
+  simp only [Iter.IsPlausibleStep, Monadic.isPlausibleStep_iff, step_eq_monadicStep]
+  constructor
+  · intro h
+    generalize hs : (step.mapIterator Iter.toIterM) = stepM at h
+    cases h
+    replace hs := congrArg (IterStep.mapIterator IterM.toIter) hs
+    simpa using hs
+  · rintro rfl
+    simp only [IterStep.mapIterator_mapIterator, Iter.toIterM_comp_toIter, IterStep.mapIterator_id]
+
+theorem Iterator.step_eq_step [UpwardEnumerable α] [LT α] [DecidableLT α]
+    {it : Iter (α := Rxo.Iterator α) α} :
+    it.step = ⟨Iterator.step it, isPlausibleStep_iff.mpr rfl⟩ := by
+  simp [Iter.step, step_eq_monadicStep, Monadic.step_eq_step, IterM.Step.toPure]
+
+instance Iterator.instIteratorCollect [UpwardEnumerable α] [LT α] [DecidableLT α]
+    {n : Type u → Type w} [Monad n] : IteratorCollect (Rxo.Iterator α) Id n :=
+  .defaultImplementation
+
+instance Iterator.instIteratorCollectPartial [UpwardEnumerable α] [LT α] [DecidableLT α]
+    {n : Type u → Type w} [Monad n] : IteratorCollectPartial (Rxo.Iterator α) Id n :=
+  .defaultImplementation
+
+theorem Iterator.Monadic.isPlausibleOutput_next {a}
+    [UpwardEnumerable α] [LT α] [DecidableLT α]
+    {it : IterM (α := Rxo.Iterator α) Id α} (h : it.internalState.next = some a)
+    (hP : a < it.internalState.upperBound) :
+    it.IsPlausibleOutput a := by
+  simp [IterM.IsPlausibleOutput, Monadic.isPlausibleStep_iff, Monadic.step, h, hP]
+
+theorem Iterator.Monadic.isPlausibleOutput_iff
+    [UpwardEnumerable α] [LT α] [DecidableLT α]
+    {it : IterM (α := Rxo.Iterator α) Id α} :
+    it.IsPlausibleOutput a ↔
+      it.internalState.next = some a ∧
+        a < it.internalState.upperBound := by
+  simp [IterM.IsPlausibleOutput, isPlausibleStep_iff, Monadic.step]
+  split
+  · simp [*]
+  · constructor
+    · rintro ⟨it', hit'⟩
+      split at hit' <;> simp_all
+    · rename_i heq
+      rintro ⟨heq', h'⟩
+      simp only [heq', Option.some.injEq] at heq
+      simp_all
+
+theorem Iterator.isPlausibleOutput_next
+    [UpwardEnumerable α] [LT α] [DecidableLT α]
+    {it : Iter (α := Rxo.Iterator α) α} (h : it.internalState.next = some a)
+    (hP : a < it.internalState.upperBound) :
+    it.IsPlausibleOutput a := by
+  simp [Iter.IsPlausibleOutput, Monadic.isPlausibleOutput_iff, Iter.toIterM, h, hP]
+
+theorem Iterator.isPlausibleOutput_iff
+    [UpwardEnumerable α] [LT α] [DecidableLT α]
+    {it : Iter (α := Rxo.Iterator α) α} :
+    it.IsPlausibleOutput a ↔
+      it.internalState.next = some a ∧
+        a < it.internalState.upperBound := by
+  simp [Iter.IsPlausibleOutput, Monadic.isPlausibleOutput_iff, Iter.toIterM]
+
+theorem Iterator.Monadic.isPlausibleSuccessorOf_iff
+    [UpwardEnumerable α] [LT α] [DecidableLT α]
+    {it' it : IterM (α := Rxo.Iterator α) Id α} :
+    it'.IsPlausibleSuccessorOf it ↔
+      ∃ a, it.internalState.next = some a ∧
+        a < it.internalState.upperBound ∧
+        UpwardEnumerable.succ? a = it'.internalState.next ∧
+        it'.internalState.upperBound = it.internalState.upperBound := by
+  simp only [IterM.IsPlausibleSuccessorOf]
+  constructor
+  · rintro ⟨step, h, h'⟩
+    cases h'
+    simp only [Monadic.step] at h
+    split at h
+    · cases h
+    · split at h
+      · simp only [IterStep.successor, Option.some.injEq] at h
+        cases h
+        exact ⟨_, ‹_›, ‹_›, rfl, rfl⟩
+      · cases h
+  · rintro ⟨a, h, hP, h'⟩
+    refine ⟨.yield it' a, rfl, ?_⟩
+    simp only [IterM.IsPlausibleStep, Iterator.IsPlausibleStep, step, h, hP, ↓reduceIte,
+      IterStep.yield.injEq, and_true]
+    simp [h'.1, ← h'.2]
+
+theorem Iterator.isPlausibleSuccessorOf_iff
+    [UpwardEnumerable α] [LT α] [DecidableLT α]
+    {it' it : Iter (α := Rxo.Iterator α) α} :
+    it'.IsPlausibleSuccessorOf it ↔
+      ∃ a, it.internalState.next = some a ∧
+        a < it.internalState.upperBound ∧
+        UpwardEnumerable.succ? a = it'.internalState.next ∧
+        it'.internalState.upperBound = it.internalState.upperBound := by
+  simp [Iter.IsPlausibleSuccessorOf, Monadic.isPlausibleSuccessorOf_iff, Iter.toIterM]
+
+theorem Iterator.isSome_next_of_isPlausibleIndirectOutput
+    [UpwardEnumerable α] [LT α] [DecidableLT α]
+    {it : Iter (α := Rxo.Iterator α) α} {out : α} (h : it.IsPlausibleIndirectOutput out) :
+    it.internalState.next.isSome := by
+  cases h
+  case direct h =>
+    rw [isPlausibleOutput_iff] at h
+    simp [h]
+  case indirect h _ =>
+    rw [isPlausibleSuccessorOf_iff] at h
+    obtain ⟨a, ha, _⟩ := h
+    simp [ha]
+
+private def List.Sublist.filter_mono {l : List α} {P Q : α → Bool} (h : ∀ a, P a → Q a) :
+    List.Sublist (l.filter P) (l.filter Q) := by
+  apply List.Sublist.trans (l₂ := (l.filter Q).filter P)
+  · simp [Bool.and_eq_left_iff_imp.mpr (h _)]
+  · apply List.filter_sublist
+
+private def List.length_filter_strict_mono {l : List α} {P Q : α → Bool} {a : α}
+    (h : ∀ a, P a → Q a) (ha : a ∈ l) (hPa : ¬ P a) (hQa : Q a) :
+    (l.filter P).length < (l.filter Q).length := by
+  have hsl : List.Sublist (l.filter P) (l.filter Q) := by
+    apply List.Sublist.filter_mono
+    exact h
+  apply Nat.lt_of_le_of_ne
+  · apply List.Sublist.length_le
+    exact hsl
+  · intro h
+    apply hPa
+    have heq := List.Sublist.eq_of_length hsl h
+    have : a ∈ List.filter Q l := List.mem_filter.mpr ⟨ha, hQa⟩
+    rw [← heq, List.mem_filter] at this
+    exact this.2
+
+private def Iterator.instFinitenessRelation [UpwardEnumerable α] [LT α] [DecidableLT α]
+    [LawfulUpwardEnumerable α] [Rxo.IsAlwaysFinite α] :
+    FinitenessRelation (Rxo.Iterator α) Id where
+  rel it' it := it'.IsPlausibleSuccessorOf it
+  wf := by
+    constructor
+    intro it
+    have hnone : ∀ bound, Acc (fun it' it : IterM (α := Rxo.Iterator α) Id α => it'.IsPlausibleSuccessorOf it)
+        ⟨⟨none, bound⟩⟩ := by
+      intro bound
+      constructor
+      intro it' ⟨step, hs₁, hs₂⟩
+      simp only [IterM.IsPlausibleStep, Iterator.IsPlausibleStep, Monadic.step] at hs₂
+      simp [hs₂, IterStep.successor] at hs₁
+    simp only [IterM.IsPlausibleSuccessorOf, IterM.IsPlausibleStep, Iterator.IsPlausibleStep,
+      Monadic.step, exists_eq_right] at hnone ⊢
+    match it with
+    | ⟨⟨none, _⟩⟩ => apply hnone
+    | ⟨⟨some init, bound⟩⟩ =>
+      obtain ⟨n, hn⟩ := Rxo.IsAlwaysFinite.finite init bound
+      induction n generalizing init with
+      | zero =>
+        simp only [succMany?_zero, Option.elim_some] at hn
+        constructor
+        simp [hn, IterStep.successor]
+      | succ n ih =>
+        constructor
+        rintro it'
+        simp only [succMany?_succ?_eq_succ?_bind_succMany?] at hn
+        match hs : succ? init with
+        | none =>
+          simp only [hs]
+          intro h
+          split at h
+          · cases h
+            apply hnone
+          · cases h
+        | some a =>
+          intro h
+          simp only [hs] at h hn
+          specialize ih _ hn
+          split at h
+          · cases h
+            exact ih
+          · cases h
+  subrelation := id
+
+@[no_expose]
+instance Iterator.instFinite [UpwardEnumerable α] [LT α] [DecidableLT α]
+    [LawfulUpwardEnumerable α] [Rxo.IsAlwaysFinite α] :
+    Finite (Rxo.Iterator α) Id :=
+  .of_finitenessRelation instFinitenessRelation
+
+private def Iterator.instProductivenessRelation [UpwardEnumerable α] [LT α] [DecidableLT α]
+    [LawfulUpwardEnumerable α] :
+    ProductivenessRelation (Rxo.Iterator α) Id where
+  rel := emptyWf.rel
+  wf := emptyWf.wf
+  subrelation {it it'} h := by
+    exfalso
+    simp only [IterM.IsPlausibleSkipSuccessorOf, IterM.IsPlausibleStep,
+      Iterator.IsPlausibleStep, Monadic.step] at h
+    split at h
+    · cases h
+    · split at h
+      · cases h
+      · cases h
+
+@[no_expose]
+instance Iterator.instProductive [UpwardEnumerable α] [LT α] [DecidableLT α]
+    [LawfulUpwardEnumerable α] :
+    Productive (Rxo.Iterator α) Id :=
+  .of_productivenessRelation instProductivenessRelation
+
+instance Iterator.instIteratorAccess [UpwardEnumerable α] [LT α] [DecidableLT α]
+    [LawfulUpwardEnumerable α] [LawfulUpwardEnumerableLT α] [Trans (α := α) (· < ·) (· < ·) (· < ·)] :
+    IteratorAccess (Rxo.Iterator α) Id where
+  nextAtIdx? it n := ⟨match it.internalState.next.bind (UpwardEnumerable.succMany? n) with
+    | none => .done
+    | some next => if next < it.internalState.upperBound then
+        .yield ⟨⟨UpwardEnumerable.succ? next, it.internalState.upperBound⟩⟩ next
+      else
+        .done, (by
+      induction n generalizing it
+      · split <;> rename_i heq
+        · apply IterM.IsPlausibleNthOutputStep.done
+          simp only [Monadic.isPlausibleStep_iff, Monadic.step]
+          simp only [Option.bind_eq_none_iff, succMany?_zero, reduceCtorEq,
+            imp_false] at heq
+          cases heq' : it.internalState.next
+          · simp
+          · rw [heq'] at heq
+            exfalso
+            exact heq _ rfl
+        · cases heq' : it.internalState.next
+          · simp [heq'] at heq
+          simp only [heq', Option.bind_some, succMany?_zero, Option.some.injEq] at heq
+          cases heq
+          split <;> rename_i heq''
+          · apply IterM.IsPlausibleNthOutputStep.zero_yield
+            simp [Monadic.isPlausibleStep_iff, Monadic.step, heq', heq'']
+          · apply IterM.IsPlausibleNthOutputStep.done
+            simp [Monadic.isPlausibleStep_iff, Monadic.step, heq', heq'']
+      · rename_i n ih
+        split <;> rename_i heq
+        · cases heq' : it.internalState.next
+          · apply IterM.IsPlausibleNthOutputStep.done
+            simp only [Monadic.isPlausibleStep_iff, Monadic.step, heq']
+          · rename_i out
+            simp only [heq', Option.bind_some, succMany?_succ?_eq_succ?_bind_succMany?] at heq
+            specialize ih ⟨⟨UpwardEnumerable.succ? out, it.internalState.upperBound⟩⟩
+            simp only [heq] at ih
+            by_cases heq'' : out < it.internalState.upperBound
+            · apply IterM.IsPlausibleNthOutputStep.yield
+              · simp only [Monadic.isPlausibleStep_iff, Monadic.step, heq', heq'', ↓reduceIte,
+                IterStep.yield.injEq]
+                exact ⟨rfl, rfl⟩
+              · exact ih
+            · apply IterM.IsPlausibleNthOutputStep.done
+              simp [Monadic.isPlausibleStep_iff, Monadic.step, heq', heq'']
+        · cases heq' : it.internalState.next
+          · simp [heq'] at heq
+          rename_i out
+          simp only [heq', Option.bind_some] at heq
+          have hlt : UpwardEnumerable.LT out _ := ⟨n, heq⟩
+          simp only [succMany?_succ?_eq_succ?_bind_succMany?] at heq
+          specialize ih ⟨⟨UpwardEnumerable.succ? out, it.internalState.upperBound⟩⟩
+          simp only [heq] at ih
+          by_cases hout : out < it.internalState.upperBound
+          · apply IterM.IsPlausibleNthOutputStep.yield
+            · simp only [Monadic.isPlausibleStep_iff, Monadic.step, heq', hout, ↓reduceIte,
+              IterStep.yield.injEq]
+              exact ⟨rfl, rfl⟩
+            · apply ih
+          · rename_i next
+            have := hout.imp (fun h : next < it.internalState.upperBound => by
+              rw [← UpwardEnumerable.lt_iff] at hlt
+              exact Trans.trans hlt h)
+            simp only [this, ↓reduceIte]
+            simp only [this, ↓reduceIte] at ih
+            apply IterM.IsPlausibleNthOutputStep.done
+            simp [Monadic.isPlausibleStep_iff, Monadic.step, heq', hout])⟩
+
+instance Iterator.instLawfulDeterministicIterator [UpwardEnumerable α] [LT α] [DecidableLT α] :
+    LawfulDeterministicIterator (Rxo.Iterator α) Id where
+  isPlausibleStep_eq_eq it := ⟨Monadic.step it, rfl⟩
+
+theorem Iterator.Monadic.isPlausibleIndirectOutput_iff
+    [UpwardEnumerable α] [LT α] [DecidableLT α] [LawfulUpwardEnumerableLT α]
+    [LawfulUpwardEnumerable α] [Trans (α := α) (· < ·) (· < ·) (· < ·)]
+    {it : IterM (α := Rxo.Iterator α) Id α} {out : α} :
+    it.IsPlausibleIndirectOutput out ↔
+      ∃ n, it.internalState.next.bind (succMany? n ·) = some out ∧
+        out < it.internalState.upperBound := by
+  constructor
+  · intro h
+    induction h
+    case direct h =>
+      rw [Monadic.isPlausibleOutput_iff] at h
+      refine ⟨0, by simp [h, LawfulUpwardEnumerable.succMany?_zero]⟩
+    case indirect h _ ih =>
+      rw [Monadic.isPlausibleSuccessorOf_iff] at h
+      obtain ⟨n, hn⟩ := ih
+      obtain ⟨a, ha, h₁, h₂, h₃⟩ := h
+      refine ⟨n + 1, ?_⟩
+      simp [ha, ← h₃, hn.2, succMany?_succ?_eq_succ?_bind_succMany?, h₂, hn]
+  · rintro ⟨n, hn, hu⟩
+    induction n generalizing it
+    case zero =>
+      apply IterM.IsPlausibleIndirectOutput.direct
+      rw [Monadic.isPlausibleOutput_iff]
+      exact ⟨by simpa [LawfulUpwardEnumerable.succMany?_zero] using hn, hu⟩
+    case succ ih =>
+      cases hn' : it.internalState.next
+      · simp [hn'] at hn
+      rename_i a
+      simp only [hn', Option.bind_some] at hn
+      have hlt : UpwardEnumerable.LT a out := ⟨_, hn⟩
+      rw [succMany?_succ?_eq_succ?_bind_succMany?] at hn
+      cases hn' : succ? a
+      · simp only [hn', Option.bind_none, reduceCtorEq] at hn
+      rename_i a'
+      simp only [hn', Option.bind_some] at hn
+      specialize ih (it := ⟨some a', it.internalState.upperBound⟩) hn hu
+      refine IterM.IsPlausibleIndirectOutput.indirect ?_ ih
+      rw [Monadic.isPlausibleSuccessorOf_iff]
+      refine ⟨a, ‹_›, ?_, hn', rfl⟩
+      exact Trans.trans (α := α) (UpwardEnumerable.lt_iff.mpr hlt) hu
+
+theorem Iterator.isPlausibleIndirectOutput_iff
+    [UpwardEnumerable α] [LT α] [DecidableLT α] [Trans (α := α) (· < ·) (· < ·) (· < ·)]
+    [LawfulUpwardEnumerable α] [LawfulUpwardEnumerableLT α]
+    {it : Iter (α := Rxo.Iterator α) α} {out : α} :
+    it.IsPlausibleIndirectOutput out ↔
+      ∃ n, it.internalState.next.bind (succMany? n ·) = some out ∧
+        out < it.internalState.upperBound := by
+  simp only [Iter.isPlausibleIndirectOutput_iff_isPlausibleIndirectOutput_toIterM,
+    Monadic.isPlausibleIndirectOutput_iff, Iter.toIterM]
+
+section IteratorLoop
+
+/-!
+## Efficient `IteratorLoop` instance
+As long as the compiler cannot optimize away the `Option` in the internal state, we use a special
+loop implementation.
+-/
+
+@[always_inline, inline]
+instance Iterator.instIteratorLoop [UpwardEnumerable α] [LT α] [DecidableLT α]
+    [LawfulUpwardEnumerable α] [LawfulUpwardEnumerableLT α] [Trans (α := α) (· < ·) (· < ·) (· < ·)]
+    {n : Type u → Type w} [Monad n] :
+    IteratorLoop (Rxo.Iterator α) Id n where
+  forIn _ γ Pl wf it init f :=
+    match it with
+    | ⟨⟨some next, upperBound⟩⟩ =>
+      if hu : next < upperBound then
+        loop γ Pl wf upperBound next init (fun a ha₁ ha₂ c => f a ?hf c) next ?hle hu
+      else
+        return init
+    | ⟨⟨none, _⟩⟩ => return init
+  where
+    @[specialize]
+    loop γ Pl wf (upperBound : α) least acc
+        (f : (out : α) → UpwardEnumerable.LE least out → out < upperBound → (c : γ) → n (Subtype (fun s : ForInStep γ => Pl out c s)))
+        (next : α) (hl : UpwardEnumerable.LE least next) (hu : next < upperBound) : n γ := do
+      match ← f next hl hu acc with
+      | ⟨.yield acc', _⟩ =>
+        match hs : UpwardEnumerable.succ? next with
+        | some next' =>
+          if hu : next' < upperBound then
+            loop γ Pl wf upperBound least acc' f next' ?hle' hu
+          else
+            return acc'
+        | none => return acc'
+      | ⟨.done acc', _⟩ => return acc'
+    termination_by IteratorLoop.WithWF.mk ⟨⟨some next, upperBound⟩⟩ acc (hwf := wf)
+    decreasing_by
+      simp [IteratorLoop.rel, Monadic.isPlausibleStep_iff,
+        Monadic.step, *]
+  finally
+    case hf =>
+      rw [Monadic.isPlausibleIndirectOutput_iff]
+      obtain ⟨n, hn⟩ := ha₁
+      exact ⟨n, hn, ha₂⟩
+    case hle =>
+      exact UpwardEnumerable.le_refl _
+    case hle' =>
+      refine UpwardEnumerable.le_trans hl ⟨1, ?_⟩
+      simp [succMany?_one, hs]
+
+partial instance Iterator.instIteratorLoopPartial [UpwardEnumerable α] [LT α] [DecidableLT α]
+    [LawfulUpwardEnumerable α] [LawfulUpwardEnumerableLT α] [Trans (α := α) (· < ·) (· < ·) (· < ·)]
+    {n : Type u → Type w} [Monad n] : IteratorLoopPartial (Rxo.Iterator α) Id n where
+  forInPartial _ γ it init f :=
+    match it with
+    | ⟨⟨some next, upperBound⟩⟩ =>
+      if hu : next < upperBound then
+        loop γ upperBound next init (fun a ha₁ ha₂ c => f a ?hf c) next ?hle hu
+      else
+        return init
+    | ⟨⟨none, _⟩⟩ => return init
+  where
+    @[specialize]
+    loop γ (upperBound : α) least acc
+        (f : (out : α) → UpwardEnumerable.LE least out → out < upperBound → (c : γ) → n (ForInStep γ))
+        (next : α) (hl : UpwardEnumerable.LE least next) (hu : next < upperBound) : n γ := do
+      match ← f next hl hu acc with
+      | .yield acc' =>
+        match hs : succ? next with
+        | some next' =>
+          if hu : next' < upperBound then
+            loop γ upperBound least acc' f next' ?hle' hu
+          else
+            return acc'
+        | none => return acc'
+      | .done acc' => return acc'
+  finally
+    case hf =>
+      rw [Monadic.isPlausibleIndirectOutput_iff]
+      obtain ⟨n, hn⟩ := ha₁
+      exact ⟨n, hn, ha₂⟩
+    case hle =>
+      exact UpwardEnumerable.le_refl _
+    case hle' =>
+      refine UpwardEnumerable.le_trans hl ⟨1, ?_⟩
+      simp [succMany?_one, hs]
+
+theorem Iterator.instIteratorLoop.loop_eq [UpwardEnumerable α] [LT α] [DecidableLT α]
+    [LawfulUpwardEnumerable α] [LawfulUpwardEnumerableLT α] [Trans (α := α) (· < ·) (· < ·) (· < ·)]
+    {n : Type u → Type w} [Monad n] [LawfulMonad n] {γ : Type u}
+    {lift} [Internal.LawfulMonadLiftBindFunction lift]
+    {PlausibleForInStep} {upperBound} {next} {hl} {hu} {f} {acc} {wf} :
+    loop (α := α) (n := n) γ PlausibleForInStep wf upperBound least acc f next hl hu =
+      (do
+        match ← f next hl hu acc with
+        | ⟨.yield c, _⟩ =>
+          letI it' : IterM (α := Rxo.Iterator α) Id α := ⟨⟨succ? next, upperBound⟩⟩
+          IterM.DefaultConsumers.forIn' (m := Id) lift γ
+            PlausibleForInStep wf it' c it'.IsPlausibleIndirectOutput (fun _ => id)
+            (fun b h c => f b
+                (by
+                  refine UpwardEnumerable.le_trans hl ?_
+                  simp only [Monadic.isPlausibleIndirectOutput_iff, it',
+                    ← succMany?_succ?_eq_succ?_bind_succMany?] at h
+                  exact ⟨h.choose + 1, h.choose_spec.1⟩)
+                (by
+                  simp only [Monadic.isPlausibleIndirectOutput_iff, it'] at h
+                  exact h.choose_spec.2) c)
+        | ⟨.done c, _⟩ => return c) := by
+  rw [loop]
+  apply bind_congr
+  intro step
+  split
+  · split
+    · split
+      · simp only [*]
+        rw [IterM.DefaultConsumers.forIn']
+        simp only [Monadic.step_eq_step, Monadic.step, ↓reduceIte, *,
+          Internal.LawfulMonadLiftBindFunction.liftBind_pure]
+        rw [loop_eq (lift := lift)]
+        apply bind_congr
+        intro step
+        split
+        · apply IterM.DefaultConsumers.forIn'_eq_forIn'
+          intros; rfl
+        · simp
+      · simp only [*]
+        rw [IterM.DefaultConsumers.forIn']
+        simp [Monadic.step_eq_step, Monadic.step, *,
+          Internal.LawfulMonadLiftBindFunction.liftBind_pure]
+    · simp only [*]
+      rw [IterM.DefaultConsumers.forIn']
+      simp [Monadic.step_eq_step, Monadic.step, Internal.LawfulMonadLiftBindFunction.liftBind_pure]
+  · simp
+termination_by IteratorLoop.WithWF.mk ⟨⟨some next, upperBound⟩⟩ acc (hwf := wf)
+decreasing_by
+      simp [IteratorLoop.rel, Monadic.isPlausibleStep_iff, Monadic.step, *]
+
+instance Iterator.instLawfulIteratorLoop [UpwardEnumerable α] [LT α] [DecidableLT α]
+    [LawfulUpwardEnumerable α] [LawfulUpwardEnumerableLT α] [Trans (α := α) (· < ·) (· < ·) (· < ·)]
+    {n : Type u → Type w} [Monad n] [LawfulMonad n] :
+    LawfulIteratorLoop (Rxo.Iterator α) Id n where
+  lawful := by
+    intro lift instLawfulMonadLiftFunction
+    ext γ PlausibleForInStep hwf it init f
+    simp only [IteratorLoop.forIn, IteratorLoop.defaultImplementation]
+    rw [IterM.DefaultConsumers.forIn']
+    simp only [Monadic.step_eq_step, Monadic.step]
+    simp only [Internal.LawfulMonadLiftBindFunction.liftBind_pure]
+    split
+    · rename_i it f next upperBound f'
+      simp
+      split
+      · simp only
+        rw [instIteratorLoop.loop_eq (lift := lift)]
+        apply bind_congr
+        intro step
+        split
+        · apply IterM.DefaultConsumers.forIn'_eq_forIn'
+          intro b c hPb hQb
+          congr
+        · simp
+      · simp
+    · simp
+
+end IteratorLoop
+
+end Rxo
+
+namespace Rxi
+
+variable {α : Type u} {lo a : α}
+
+/-- Internal state of the range iterators. Do not depend on its internals. -/
+@[unbox]
+protected structure Iterator (α : Type u) where
+  next : Option α
+
+/--
+The pure function mapping a range iterator of type `IterM` to the next step of the iterator.
+
+This function is prefixed with `Monadic` in order to disambiguate it from the version for iterators
+of type `Iter`.
+-/
+@[inline]
+def Iterator.Monadic.step [UpwardEnumerable α]
+    (it : IterM (α := Rxi.Iterator α) Id α) :
+    IterStep (IterM (α := Rxi.Iterator α) Id α) α :=
+  match it.internalState.next with
+  | none => .done
+  | some next => .yield ⟨⟨UpwardEnumerable.succ? next⟩⟩ next
+
+/--
+The pure function mapping a range iterator of type `Iter` to the next step of the iterator.
+-/
+@[always_inline, inline]
+def Iterator.step [UpwardEnumerable α]
+    (it : Iter (α := Rxi.Iterator α) α) :
+    IterStep (Iter (α := Rxi.Iterator α) α) α :=
+  match it.internalState.next with
+  | none => .done
+  | some next => .yield ⟨⟨UpwardEnumerable.succ? next⟩⟩ next
+
+theorem Iterator.step_eq_monadicStep [UpwardEnumerable α]
+    {it : Iter (α := Rxi.Iterator α) α} :
+    Iterator.step it = (Iterator.Monadic.step it.toIterM).mapIterator IterM.toIter := by
+  simp only [step, Monadic.step, Iter.toIterM]
+  split <;> rfl
+
+@[always_inline, inline]
+instance [UpwardEnumerable α] :
+    Iterator (Rxi.Iterator α) Id α where
+  IsPlausibleStep it step := step = Iterator.Monadic.step it
+  step it := pure ⟨Iterator.Monadic.step it, rfl⟩
+
+theorem Iterator.Monadic.isPlausibleStep_iff [UpwardEnumerable α]
+    {it : IterM (α := Rxi.Iterator α) Id α} {step} :
+    it.IsPlausibleStep step ↔ step = Iterator.Monadic.step it := by
+  exact Iff.rfl
+
+theorem Iterator.Monadic.step_eq_step [UpwardEnumerable α]
+    {it : IterM (α := Rxi.Iterator α) Id α} :
+    it.step = pure ⟨Iterator.Monadic.step it, isPlausibleStep_iff.mpr rfl⟩ := by
+  simp [IterM.step, Iterators.Iterator.step]
+
+theorem Iterator.isPlausibleStep_iff [UpwardEnumerable α]
+    {it : Iter (α := Rxi.Iterator α) α} {step} :
+    it.IsPlausibleStep step ↔ step = Iterator.step it := by
+  simp only [Iter.IsPlausibleStep, Monadic.isPlausibleStep_iff, step_eq_monadicStep]
+  constructor
+  · intro h
+    generalize hs : (step.mapIterator Iter.toIterM) = stepM at h
+    cases h
+    replace hs := congrArg (IterStep.mapIterator IterM.toIter) hs
+    simpa using hs
+  · rintro rfl
+    simp only [IterStep.mapIterator_mapIterator, Iter.toIterM_comp_toIter, IterStep.mapIterator_id]
+
+theorem Iterator.step_eq_step [UpwardEnumerable α]
+    {it : Iter (α := Rxi.Iterator α) α} :
+    it.step = ⟨Iterator.step it, isPlausibleStep_iff.mpr rfl⟩ := by
+  simp [Iter.step, step_eq_monadicStep, Monadic.step_eq_step, IterM.Step.toPure]
+
+instance Iterator.instIteratorCollect [UpwardEnumerable α]
+    {n : Type u → Type w} [Monad n] : IteratorCollect (Rxi.Iterator α) Id n :=
+  .defaultImplementation
+
+instance Iterator.instIteratorCollectPartial [UpwardEnumerable α]
+    {n : Type u → Type w} [Monad n] : IteratorCollectPartial (Rxi.Iterator α) Id n :=
+  .defaultImplementation
+
+theorem Iterator.Monadic.isPlausibleOutput_next {a} [UpwardEnumerable α]
+    {it : IterM (α := Rxi.Iterator α) Id α} (h : it.internalState.next = some a) :
+    it.IsPlausibleOutput a := by
+  simp [IterM.IsPlausibleOutput, Monadic.isPlausibleStep_iff, Monadic.step, h]
+
+theorem Iterator.Monadic.isPlausibleOutput_iff
+    [UpwardEnumerable α]
+    {it : IterM (α := Rxi.Iterator α) Id α} :
+    it.IsPlausibleOutput a ↔
+      it.internalState.next = some a := by
+  simp [IterM.IsPlausibleOutput, isPlausibleStep_iff, Monadic.step]
+  split
+  · simp [*]
+  · simp_all [eq_comm (a := a)]
+
+theorem Iterator.isPlausibleOutput_next
+    [UpwardEnumerable α]
+    {it : Iter (α := Rxi.Iterator α) α} (h : it.internalState.next = some a) :
+    it.IsPlausibleOutput a := by
+  simp [Iter.IsPlausibleOutput, Monadic.isPlausibleOutput_iff, Iter.toIterM, h]
+
+theorem Iterator.isPlausibleOutput_iff
+    [UpwardEnumerable α]
+    {it : Iter (α := Rxi.Iterator α) α} :
+    it.IsPlausibleOutput a ↔
+      it.internalState.next = some a := by
+  simp [Iter.IsPlausibleOutput, Monadic.isPlausibleOutput_iff, Iter.toIterM]
+
+theorem Iterator.Monadic.isPlausibleSuccessorOf_iff
+    [UpwardEnumerable α]
+    {it' it : IterM (α := Rxi.Iterator α) Id α} :
+    it'.IsPlausibleSuccessorOf it ↔
+      ∃ a, it.internalState.next = some a ∧
+        UpwardEnumerable.succ? a = it'.internalState.next := by
+  simp only [IterM.IsPlausibleSuccessorOf]
+  constructor
+  · rintro ⟨step, h, h'⟩
+    cases h'
+    simp only [Monadic.step] at h
+    split at h
+    · cases h
+    · cases h
+      simp_all
+  · rintro ⟨a, h, h'⟩
+    refine ⟨.yield it' a, rfl, ?_⟩
+    simp only [IterM.IsPlausibleStep, Iterator.IsPlausibleStep, step, h,
+      IterStep.yield.injEq, and_true]
+    simp [h']
+
+theorem Iterator.isPlausibleSuccessorOf_iff
+    [UpwardEnumerable α]
+    {it' it : Iter (α := Rxi.Iterator α) α} :
+    it'.IsPlausibleSuccessorOf it ↔
+      ∃ a, it.internalState.next = some a ∧
+        UpwardEnumerable.succ? a = it'.internalState.next := by
+  simp [Iter.IsPlausibleSuccessorOf, Monadic.isPlausibleSuccessorOf_iff, Iter.toIterM]
+
+theorem Iterator.isSome_next_of_isPlausibleIndirectOutput
+    [UpwardEnumerable α]
+    {it : Iter (α := Rxi.Iterator α) α} {out : α} (h : it.IsPlausibleIndirectOutput out) :
+    it.internalState.next.isSome := by
+  cases h
+  case direct h =>
+    rw [isPlausibleOutput_iff] at h
+    simp [h]
+  case indirect h _ =>
+    rw [isPlausibleSuccessorOf_iff] at h
+    obtain ⟨a, ha, _⟩ := h
+    simp [ha]
+
+-- private def List.Sublist.filter_mono {l : List α} {P Q : α → Bool} (h : ∀ a, P a → Q a) :
+--     List.Sublist (l.filter P) (l.filter Q) := by
+--   apply List.Sublist.trans (l₂ := (l.filter Q).filter P)
+--   · simp [Bool.and_eq_left_iff_imp.mpr (h _)]
+--   · apply List.filter_sublist
+
+-- private def List.length_filter_strict_mono {l : List α} {P Q : α → Bool} {a : α}
+--     (h : ∀ a, P a → Q a) (ha : a ∈ l) (hPa : ¬ P a) (hQa : Q a) :
+--     (l.filter P).length < (l.filter Q).length := by
+--   have hsl : List.Sublist (l.filter P) (l.filter Q) := by
+--     apply List.Sublist.filter_mono
+--     exact h
+--   apply Nat.lt_of_le_of_ne
+--   · apply List.Sublist.length_le
+--     exact hsl
+--   · intro h
+--     apply hPa
+--     have heq := List.Sublist.eq_of_length hsl h
+--     have : a ∈ List.filter Q l := List.mem_filter.mpr ⟨ha, hQa⟩
+--     rw [← heq, List.mem_filter] at this
+--     exact this.2
+
+private def Iterator.instFinitenessRelation [UpwardEnumerable α]
+    [LawfulUpwardEnumerable α] [Rxi.IsAlwaysFinite α] :
+    FinitenessRelation (Rxi.Iterator α) Id where
+  rel it' it := it'.IsPlausibleSuccessorOf it
+  wf := by
+    constructor
+    intro it
+    have hnone : Acc (fun it' it : IterM (α := Rxi.Iterator α) Id α => it'.IsPlausibleSuccessorOf it)
+        ⟨⟨none⟩⟩ := by
+      constructor
+      intro it' ⟨step, hs₁, hs₂⟩
+      simp only [IterM.IsPlausibleStep, Iterator.IsPlausibleStep, Monadic.step] at hs₂
+      simp [hs₂, IterStep.successor] at hs₁
+    simp only [IterM.IsPlausibleSuccessorOf, IterM.IsPlausibleStep, Iterator.IsPlausibleStep,
+      Monadic.step, exists_eq_right] at hnone ⊢
+    match it with
+    | ⟨⟨none⟩⟩ => apply hnone
+    | ⟨⟨some init⟩⟩ =>
+      obtain ⟨n, hn⟩ := Rxi.IsAlwaysFinite.finite init
+      induction n generalizing init with
+      | zero => simp [succMany?_zero] at hn
+      | succ n ih =>
+        constructor
+        rintro it'
+        simp only [succMany?_succ?_eq_succ?_bind_succMany?] at hn
+        match hs : succ? init with
+        | none =>
+          simp only [hs]
+          intro h
+          cases h
+          apply hnone
+        | some a =>
+          intro h
+          simp only [hs] at h hn
+          specialize ih _ hn
+          cases h
+          exact ih
+  subrelation := id
+
+@[no_expose]
+instance Iterator.instFinite [UpwardEnumerable α]
+    [LawfulUpwardEnumerable α] [Rxi.IsAlwaysFinite α] :
+    Finite (Rxi.Iterator α) Id :=
+  .of_finitenessRelation instFinitenessRelation
+
+private def Iterator.instProductivenessRelation [UpwardEnumerable α]
+    [LawfulUpwardEnumerable α] :
+    ProductivenessRelation (Rxi.Iterator α) Id where
+  rel := emptyWf.rel
+  wf := emptyWf.wf
+  subrelation {it it'} h := by
+    exfalso
+    simp only [IterM.IsPlausibleSkipSuccessorOf, IterM.IsPlausibleStep,
+      Iterator.IsPlausibleStep, Monadic.step] at h
+    split at h <;> cases h
+
+@[no_expose]
+instance Iterator.instProductive [UpwardEnumerable α]
+    [LawfulUpwardEnumerable α] :
+    Productive (Rxi.Iterator α) Id :=
+  .of_productivenessRelation instProductivenessRelation
+
+instance Iterator.instIteratorAccess [UpwardEnumerable α]
+    [LawfulUpwardEnumerable α] :
+    IteratorAccess (Rxi.Iterator α) Id where
+  nextAtIdx? it n := ⟨match it.internalState.next.bind (UpwardEnumerable.succMany? n) with
+    | none => .done
+    | some next =>
+        .yield ⟨⟨UpwardEnumerable.succ? next⟩⟩ next, (by
+      induction n generalizing it
+      · split <;> rename_i heq
+        · apply IterM.IsPlausibleNthOutputStep.done
+          simp only [Monadic.isPlausibleStep_iff, Monadic.step]
+          simp only [Option.bind_eq_none_iff, succMany?_zero, reduceCtorEq,
+            imp_false] at heq
+          cases heq' : it.internalState.next
+          · simp
+          · rw [heq'] at heq
+            exfalso
+            exact heq _ rfl
+        · cases heq' : it.internalState.next
+          · simp [heq'] at heq
+          simp only [heq', Option.bind_some, succMany?_zero, Option.some.injEq] at heq
+          cases heq
+          · apply IterM.IsPlausibleNthOutputStep.zero_yield
+            simp [Monadic.isPlausibleStep_iff, Monadic.step, heq']
+      · rename_i n ih
+        split <;> rename_i heq
+        · cases heq' : it.internalState.next
+          · apply IterM.IsPlausibleNthOutputStep.done
+            simp only [Monadic.isPlausibleStep_iff, Monadic.step, heq']
+          · rename_i out
+            simp only [heq', Option.bind_some, succMany?_succ?_eq_succ?_bind_succMany?] at heq
+            specialize ih ⟨⟨UpwardEnumerable.succ? out⟩⟩
+            simp only [heq] at ih
+            · apply IterM.IsPlausibleNthOutputStep.yield
+              · simp only [Monadic.isPlausibleStep_iff, Monadic.step, heq',
+                IterStep.yield.injEq]
+                exact ⟨rfl, rfl⟩
+              · exact ih
+        · cases heq' : it.internalState.next
+          · simp [heq'] at heq
+          rename_i out
+          simp only [heq', Option.bind_some] at heq
+          have hlt : UpwardEnumerable.LT out _ := ⟨n, heq⟩
+          simp only [succMany?_succ?_eq_succ?_bind_succMany?] at heq
+          specialize ih ⟨⟨UpwardEnumerable.succ? out⟩⟩
+          simp only [heq] at ih
+          · apply IterM.IsPlausibleNthOutputStep.yield
+            · simp only [Monadic.isPlausibleStep_iff, Monadic.step, heq',
+              IterStep.yield.injEq]
+              exact ⟨rfl, rfl⟩
+            · apply ih)⟩
+
+instance Iterator.instLawfulDeterministicIterator [UpwardEnumerable α] :
+    LawfulDeterministicIterator (Rxi.Iterator α) Id where
+  isPlausibleStep_eq_eq it := ⟨Monadic.step it, rfl⟩
+
+theorem Iterator.Monadic.isPlausibleIndirectOutput_iff
+    [UpwardEnumerable α] [LawfulUpwardEnumerable α]
+    {it : IterM (α := Rxi.Iterator α) Id α} {out : α} :
+    it.IsPlausibleIndirectOutput out ↔
+      ∃ n, it.internalState.next.bind (succMany? n ·) = some out := by
+  constructor
+  · intro h
+    induction h
+    case direct h =>
+      rw [Monadic.isPlausibleOutput_iff] at h
+      refine ⟨0, by simp [h, LawfulUpwardEnumerable.succMany?_zero]⟩
+    case indirect h _ ih =>
+      rw [Monadic.isPlausibleSuccessorOf_iff] at h
+      obtain ⟨n, hn⟩ := ih
+      obtain ⟨a, ha, h⟩ := h
+      refine ⟨n + 1, ?_⟩
+      simp [ha, succMany?_succ?_eq_succ?_bind_succMany?, hn, h]
+  · rintro ⟨n, hn⟩
+    induction n generalizing it
+    case zero =>
+      apply IterM.IsPlausibleIndirectOutput.direct
+      rw [Monadic.isPlausibleOutput_iff]
+      simpa [LawfulUpwardEnumerable.succMany?_zero] using hn
+    case succ ih =>
+      cases hn' : it.internalState.next
+      · simp [hn'] at hn
+      rename_i a
+      simp only [hn', Option.bind_some] at hn
+      have hlt : UpwardEnumerable.LT a out := ⟨_, hn⟩
+      rw [succMany?_succ?_eq_succ?_bind_succMany?] at hn
+      cases hn' : succ? a
+      · simp only [hn', Option.bind_none, reduceCtorEq] at hn
+      rename_i a'
+      simp only [hn', Option.bind_some] at hn
+      specialize ih (it := ⟨⟨some a'⟩⟩) hn
+      refine IterM.IsPlausibleIndirectOutput.indirect ?_ ih
+      rw [Monadic.isPlausibleSuccessorOf_iff]
+      exact ⟨a, ‹_›, hn'⟩
+
+theorem Iterator.isPlausibleIndirectOutput_iff
+    [UpwardEnumerable α] [LawfulUpwardEnumerable α]
+    {it : Iter (α := Rxi.Iterator α) α} {out : α} :
+    it.IsPlausibleIndirectOutput out ↔
+      ∃ n, it.internalState.next.bind (succMany? n ·) = some out := by
+  simp only [Iter.isPlausibleIndirectOutput_iff_isPlausibleIndirectOutput_toIterM,
+    Monadic.isPlausibleIndirectOutput_iff, Iter.toIterM]
+
+section IteratorLoop
+
+/-!
+## Efficient `IteratorLoop` instance
+As long as the compiler cannot optimize away the `Option` in the internal state, we use a special
+loop implementation.
+-/
+
+@[always_inline, inline]
+instance Iterator.instIteratorLoop [UpwardEnumerable α]
+    [LawfulUpwardEnumerable α]
+    {n : Type u → Type w} [Monad n] :
+    IteratorLoop (Rxi.Iterator α) Id n where
+  forIn _ γ Pl wf it init f :=
+    match it with
+    | ⟨⟨some next⟩⟩ =>
+        loop γ Pl wf next init (fun a ha c => f a ?hf c) next ?hle
+    | ⟨⟨none⟩⟩ => return init
+  where
+    @[specialize]
+    loop γ Pl wf least acc
+        (f : (out : α) → UpwardEnumerable.LE least out → (c : γ) → n (Subtype (fun s : ForInStep γ => Pl out c s)))
+        (next : α) (hl : UpwardEnumerable.LE least next) : n γ := do
+      match ← f next hl acc with
+      | ⟨.yield acc', _⟩ =>
+        match hs : UpwardEnumerable.succ? next with
+        | some next' =>
+            loop γ Pl wf least acc' f next' ?hle'
+        | none => return acc'
+      | ⟨.done acc', _⟩ => return acc'
+    termination_by IteratorLoop.WithWF.mk ⟨⟨some next⟩⟩ acc (hwf := wf)
+    decreasing_by
+      simp [IteratorLoop.rel, Monadic.isPlausibleStep_iff,
+        Monadic.step, *]
+  finally
+    case hf =>
+      rw [Monadic.isPlausibleIndirectOutput_iff]
+      exact ha
+    case hle =>
+      exact UpwardEnumerable.le_refl _
+    case hle' =>
+      refine UpwardEnumerable.le_trans hl ⟨1, ?_⟩
+      simp [succMany?_one, hs]
+
+partial instance Iterator.instIteratorLoopPartial [UpwardEnumerable α]
+    [LawfulUpwardEnumerable α]
+    {n : Type u → Type w} [Monad n] : IteratorLoopPartial (Rxi.Iterator α) Id n where
+  forInPartial _ γ it init f :=
+    match it with
+    | ⟨⟨some next⟩⟩ => loop γ next init (fun a ha c => f a ?hf c) next ?hle
+    | ⟨⟨none⟩⟩ => return init
+  where
+    @[specialize]
+    loop γ least acc
+        (f : (out : α) → UpwardEnumerable.LE least out → (c : γ) → n (ForInStep γ))
+        (next : α) (hl : UpwardEnumerable.LE least next) : n γ := do
+      match ← f next hl acc with
+      | .yield acc' =>
+        match hs : succ? next with
+        | some next' =>
+            loop γ least acc' f next' ?hle'
+        | none => return acc'
+      | .done acc' => return acc'
+  finally
+    case hf =>
+      rw [Monadic.isPlausibleIndirectOutput_iff]
+      exact ha
+    case hle =>
+      exact UpwardEnumerable.le_refl _
+    case hle' =>
+      refine UpwardEnumerable.le_trans hl ⟨1, ?_⟩
+      simp [succMany?_one, hs]
+
+theorem Iterator.instIteratorLoop.loop_eq [UpwardEnumerable α]
+    [LawfulUpwardEnumerable α]
+    {n : Type u → Type w} [Monad n] [LawfulMonad n] {γ : Type u}
+    {lift} [Internal.LawfulMonadLiftBindFunction lift]
+    {PlausibleForInStep next hl f acc wf} :
+    loop (α := α) (n := n) γ PlausibleForInStep wf least acc f next hl =
+      (do
+        match ← f next hl acc with
+        | ⟨.yield c, _⟩ =>
+          letI it' : IterM (α := Rxi.Iterator α) Id α := ⟨⟨succ? next⟩⟩
+          IterM.DefaultConsumers.forIn' (m := Id) lift γ
+            PlausibleForInStep wf it' c it'.IsPlausibleIndirectOutput (fun _ => id)
+            (fun b h c => f b
+                (by
+                  refine UpwardEnumerable.le_trans hl ?_
+                  simp only [Monadic.isPlausibleIndirectOutput_iff, it',
+                    ← succMany?_succ?_eq_succ?_bind_succMany?] at h
+                  exact ⟨h.choose + 1, h.choose_spec⟩)
+                c)
+        | ⟨.done c, _⟩ => return c) := by
+  rw [loop]
+  apply bind_congr
+  intro step
+  split
+  · split
+    · split
+      · rename_i heq
+        cases heq
+        simp only [*]
+        rw [IterM.DefaultConsumers.forIn']
+        simp only [Monadic.step_eq_step, Monadic.step, *,
+          Internal.LawfulMonadLiftBindFunction.liftBind_pure]
+        rw [loop_eq (lift := lift)]
+        apply bind_congr
+        intro step
+        split
+        · apply IterM.DefaultConsumers.forIn'_eq_forIn'
+          intros; rfl
+        · simp
+      · rename_i heq
+        cases heq
+    · simp only [*]
+      rw [IterM.DefaultConsumers.forIn']
+      simp [Monadic.step_eq_step, Monadic.step, Internal.LawfulMonadLiftBindFunction.liftBind_pure]
+  · simp
+termination_by IteratorLoop.WithWF.mk ⟨⟨some next⟩⟩ acc (hwf := wf)
+decreasing_by
+      simp [IteratorLoop.rel, Monadic.isPlausibleStep_iff, Monadic.step, *]
+
+instance Iterator.instLawfulIteratorLoop [UpwardEnumerable α]
+    [LawfulUpwardEnumerable α] {n : Type u → Type w} [Monad n] [LawfulMonad n] :
+    LawfulIteratorLoop (Rxi.Iterator α) Id n where
+  lawful := by
+    intro lift instLawfulMonadLiftFunction
+    ext γ PlausibleForInStep hwf it init f
+    simp only [IteratorLoop.forIn, IteratorLoop.defaultImplementation]
+    rw [IterM.DefaultConsumers.forIn']
+    simp only [Monadic.step_eq_step, Monadic.step]
+    simp only [Internal.LawfulMonadLiftBindFunction.liftBind_pure]
+    split
+    · rename_i it f next upperBound f'
+      rw [instIteratorLoop.loop_eq (lift := lift)]
+      apply bind_congr
+      intro step
+      split
+      · apply IterM.DefaultConsumers.forIn'_eq_forIn'
+        intro b c hPb hQb
+        congr
+      · simp
+    · simp
+
+end IteratorLoop
+
+end Rxi
+
+end Std
